doc(computability): documentation, TODOs, and questions
Add documentation, TODOs, and questions about my proof. Still a WIP.

src/computability/GNFA.lean
@@ -1,25 +1,52 @@
 /-
+Copyright (c) 2022 Russell Emerine. All rights reserved.
+Released under Apache 2.0 license as described in the file LICENSE.
 Author: Russell Emerine
-Based on: https://courses.engr.illinois.edu/cs373/sp2013/Lectures/lec07.pdf
-TODO: write comments and TODOs, organize, etc.
 -/
 import computability.regular_expressions
 import computability.NFA
 
+/-!
+# Generalized Nondeterministic Finite Automata
+
+This file contains the definition of a Generalized Nondeterministic Finite Automaton, a state
+machine which determines whether a string (implemented as a list over an arbitrary alphabet) is in
+a regular set by evaluating the string over every possible series of regular expressions. We show 
+that GNFA's are equivalent to NFA's, and that GNFA's are equivalent to smaller GNFA's with a state
+"ripped" out. Through this mechanism, we show that NFA's are equivalent to regular expressions.
+Unlike for DFA's and NFA's, GNFA's can only be made with a `fin` as the state type.
+
+## References
+
+TODO: someone please tell me how to best cite this file?
+* <https://courses.engr.illinois.edu/cs373/sp2013/Lectures/lec07.pdf>
+-/
+
 namespace fin
 
+/-
+TODO: Is there a short way to write this inline? I want to cause a contradiction against
+a hypothesis of fin.cast_succ i = fin.last n, but ne_of_lt and is_lt don't quite work there.
+Also, maybe move to data/fin.
+-/
 theorem cast_succ_ne_last {n i} : fin.cast_succ i ≠ fin.last n :=
 begin
-  cases i with i lt,
-  unfold last,
-  simp,
-  exact ne_of_lt lt,
+  apply ne_of_lt,
+  exact is_lt i,
 end
 
 end fin
 
 universes u v
 
+/--
+A GNFA is a set of `n + 2` states and a transition function between two states. The transition
+function takes the starting state or any internal state as the first state, and the accepting
+state or any internal state as the second state. There is a transition between *all* of these
+combinations, in the form of a regular expression. When following a transition, some matching
+prefix of the input string is taken. "No transition" can be simulated by using the regular
+expression `0`, which accepts no strings.
+-/
 structure GNFA (α : Type u) (n : ℕ) :=
   (step : option (fin n) → option (fin n) → regular_expression α)
 
@@ -27,8 +54,15 @@ variables {α : Type u} {σ : Type v} {n : ℕ}
 
 namespace regular_expression
 
-theorem mem_sum (x : list α) (rs : list (regular_expression α)) :
-  (list.foldl (λ a b, a + b) 0 rs).matches x ↔ (∃ (r : regular_expression α), r ∈ rs ∧ r.matches x) :=
+/--
+A string matches the sum of a list of regular expressions if and only if there is some regular
+expression in the list that it matches. This is because the sum of regular expressions matches the
+union of their respective languages.
+
+TODO: probably move to computability/regular_expression
+-/
+theorem mem_sum_iff_exists_mem (x : list α) (rs : list (regular_expression α)) :
+  (list.sum rs).matches x ↔ (∃ (r : regular_expression α), r ∈ rs ∧ r.matches x) :=
 begin
   split,
   { rw ← rs.reverse_reverse,
@@ -39,6 +73,7 @@ begin
     },
     case cons : r rs ih {
       assume hx,
+      unfold list.sum at hx,
       simp at *,
       cases hx,
       case inl {
@@ -59,6 +94,7 @@ begin
     },
     case cons : r rs ih {
       assume hx,
+      unfold list.sum,
       simp at *,
       rcases hx with ⟨r', hr', matches⟩,
       cases hr',
@@ -79,247 +115,31 @@ end regular_expression
 
 namespace GNFA
 
+instance : inhabited (GNFA α n) := ⟨ GNFA.mk (λ _ _, 0) ⟩
+
+/--
+A `trace` of a string and an internal state of a GNFA represents a way to get to the state via
+transitions of the GNFA that match parts of the string.
+-/
 inductive trace (M : GNFA α n) : list α → fin n → Prop
 | start : ∀ {x q}, x ∈ (M.step none (some q)).matches → trace x q
 | step : ∀ {x y z} p {q}, trace y p → z ∈ (M.step (some p) (some q)).matches → x = y ++ z → trace x q
 
+/--
+An `accepts` of a string represents a way to get to the accepting state of a GNFA via transitions
+of the GNFA that match parts of the string. Since this is the definition of when a GNFA accepts
+a string, this also is how the accepting language of a GNFA is described.
+
+TODO: make description clearer
+-/
 inductive accepts (M : GNFA α n) : language α
 | start : ∀ {x}, x ∈ (M.step none none).matches → accepts x
 | step : ∀ {x y z} q, M.trace y q → z ∈ (M.step (some q) none).matches → x = y ++ z → accepts x
 
-end GNFA
-
-namespace NFA
-
-def convert (M : NFA α σ) {τ} (equiv : σ ≃ τ) : NFA α τ :=
-⟨
-  (λ p a q, M.step (equiv.inv_fun p) a (equiv.inv_fun q)),
-  (λ q, M.start (equiv.inv_fun q)),
-  (λ q, M.accept (equiv.inv_fun q))
-⟩
-
-theorem convert_correct (M : NFA α σ) {τ} (equiv : σ ≃ τ) : M.accepts = (M.convert equiv).accepts :=
-begin
-  ext,
-  split,
-  { rintros ⟨q, accept, eval⟩,
-    refine ⟨equiv.to_fun q, _, _⟩,
-    { unfold convert,
-      rw set.mem_def at *,
-      simpa,
-    },
-    { clear accept,
-      revert eval,
-      rw ← x.reverse_reverse,
-      induction x.reverse generalizing q,
-      case nil {
-        assume hx,
-        unfold convert,
-        rw set.mem_def at *,
-        simpa,
-      },
-      case cons : a as ih {
-        assume hx,
-        simp at *,
-        rw NFA.mem_step_set at *,
-        rcases hx with ⟨p, mem, step⟩,
-        refine ⟨equiv.to_fun p, ih p mem, _⟩,
-        unfold convert,
-        rw set.mem_def at *,
-        simpa,
-      },
-    },        
-  },
-  { rintros ⟨q, accept, eval⟩,
-    refine ⟨equiv.inv_fun q, accept, _⟩,
-    clear accept,
-    revert eval,
-    rw ← x.reverse_reverse,
-    induction x.reverse generalizing q,
-    case nil {
-      assume hx,
-      exact hx,
-    },
-    case cons : a as ih {
-      assume hx,
-      simp at *,
-      rw NFA.mem_step_set at *,
-      rcases hx with ⟨p, mem, step⟩,
-      exact ⟨equiv.inv_fun p, ih p mem, step⟩,
-    },
-  },
-end
-
-variables
-  (M : NFA α (fin n))
-  [dec_start : decidable_pred M.start]
-  [dec_accept : decidable_pred M.accept]
-  [dec_step : ∀ p a q, decidable (M.step p a q)]
-  (as : list α)
-  (univ : ∀ a, a ∈ as)
-
-include dec_start dec_accept dec_step univ
-
-def to_GNFA : GNFA α n :=
-⟨
-  λ p q,
-  match (p, q) with
-  | (none, none) := 0
-  | (none, some q) := if M.start q then 1 else 0
-  | (some p, none) := if M.accept p then 1 else 0
-  | (some p, some q) :=
-    list.foldl (λ a b, a + b) 0 $
-      list.map (λ a, regular_expression.char a) $
-        list.filter (λ a, M.step p a q) as
-  end
-⟩
-
-theorem to_GNFA_correct : M.accepts = (M.to_GNFA as univ).accepts :=
-begin
-  ext,
-  split,
-  { rintros ⟨q, accept, eval⟩,
-    refine GNFA.accepts.step q _ _ x.append_nil.symm,
-    swap,
-    { rw set.mem_def,
-      unfold to_GNFA,
-      simp,
-      unfold to_GNFA._match_1,
-      rw set.mem_def at accept,
-      simp [accept],
-      exact rfl,
-    },
-    clear accept,
-    revert eval,
-    rw ← x.reverse_reverse,
-    induction x.reverse generalizing q,
-    case nil {
-      assume hx,
-      simp,
-      refine GNFA.trace.start _,
-      unfold to_GNFA,
-      simp,
-      unfold to_GNFA._match_1,
-      rw set.mem_def at hx,
-      simp at hx,
-      simp [hx],
-    },
-    case cons : a as ih {
-      assume hx,
-      simp at *,
-      rw NFA.mem_step_set at hx,
-      rcases hx with ⟨p, mem, step⟩,
-      refine GNFA.trace.step p (ih p mem) _ rfl,
-      rw set.mem_def,
-      unfold to_GNFA,
-      simp,
-      unfold to_GNFA._match_1,
-      rw regular_expression.mem_sum,      
-      refine ⟨regular_expression.char a, _, rfl⟩,
-      simpa [univ],
-    },
-  },
-  { assume hx,
-    cases hx with x step x y z q t step eq,
-    case start { cases step,},
-    unfold to_GNFA at step,
-    rw set.mem_def at step,
-    simp at step,
-    unfold to_GNFA._match_1 at step,
-    by_cases M.accept q,
-    swap, simp [h] at step, cases step,
-    simp [h] at step,
-    cases step,
-    refine ⟨q, h, _⟩,
-    simp at eq, cases eq,
-    clear h eq step,
-    revert t,
-    rw ← x.reverse_reverse,
-    induction x.reverse generalizing q,
-    case nil {
-      assume hx,
-      simp at *,
-      cases hx,
-      case start : x step {
-        unfold to_GNFA at step,
-        rw set.mem_def at step,
-        simp at step,
-        unfold to_GNFA._match_1 at step,
-        by_cases M.start x,
-        exact h,
-        simp [h] at step,
-        cases step,
-      },
-      case step : x y z p t step eq {
-        simp at eq,
-        rw eq.2 at *,
-        unfold to_GNFA at step,
-        rw set.mem_def at step,
-        simp at step,
-        unfold to_GNFA._match_1 at step,
-        rw regular_expression.mem_sum at step,
-        rcases step with ⟨r, mem, matches⟩,
-        simp at mem,
-        rcases mem with ⟨a, _, eq⟩,
-        rw ← eq at matches,
-        cases matches,
-      },
-    },
-    case cons : a as ih {
-      assume hx,
-      simp at *,
-      rw NFA.mem_step_set,
-      cases hx,
-      case start : q step {
-        unfold to_GNFA at step,
-        simp at step,
-        rw set.mem_def at step,
-        unfold to_GNFA._match_1 at step,
-        by_cases M.start q,
-        { simp [h] at step,
-          by_cases as.reverse.append [a] = [],
-          { have h : as.reverse ++ [a] = list.nil := h,
-            rw ← list.reverse_cons a as at h,
-            rw list.reverse_eq_nil at h,
-            contradiction,
-          },
-          { rcases list.exists_cons_of_ne_nil h with ⟨a, as, h⟩,
-            rw h at step,
-            cases step,
-          },
-        },
-        { simp [h] at step,
-          cases step,
-        },
-      },
-      case step : y z p q t step eq {
-        unfold to_GNFA at step,
-        rw set.mem_def at step,
-        simp at step,
-        unfold to_GNFA._match_1 at step,
-        replace eq : as.reverse ++ [a] = y ++ z := eq,
-        rw regular_expression.mem_sum at step,
-        rcases step with ⟨r, mem, matches⟩,
-        simp at mem,
-        rcases mem with ⟨b, ⟨_, step⟩, eq⟩,
-        rw ← eq at matches,
-        cases matches,
-        rw ← list.reverse_inj at eq,
-        simp at eq,
-        rw ← eq.1 at step,
-        refine ⟨p, _, step⟩,
-        rw ← y.reverse_reverse at t,
-        rw ← eq.2 at t,
-        exact ih p t,        
-      },
-    },
-  },
-end
-
-end NFA
-
-namespace GNFA
-
+/--
+"Rips" an internal state out of a GNFA, making it smaller by one without changing its accepting
+language.
+-/
 def rip (M : GNFA α n.succ) : GNFA α n :=
 ⟨
   λ p q,
@@ -542,6 +362,7 @@ begin
   },
 end
 
+/- TODO: maybe mark as @simp -/
 theorem rip_correct (M : GNFA α n.succ) : M.rip.accepts = M.accepts :=
 begin
   ext,
@@ -668,6 +489,11 @@ begin
   },
 end
 
+/--
+Convert a GNA to a regular expression by repeatedly removing internal states. When there are no
+internal states left, there will only be one transition, from the starting state to the accepting
+state. Its regular expression will accept the same language as the original GNFA.
+-/
 def to_regular_expression : Π {n}, GNFA α n → regular_expression α
 | 0 M := M.step none none
 | (nat.succ n) M := M.rip.to_regular_expression
@@ -702,15 +528,269 @@ end GNFA
 
 namespace NFA
 
-theorem to_regular_expression (M : NFA α σ) [fintype α] [fintype σ] : ∃ (r : regular_expression α), M.accepts = r.matches :=
+/--
+Given an equivalence between `σ` and `τ`, convert an NFA with state type `σ` into the corresponding
+NFA with state type `τ`.
+
+TODO: possibly move to computability/NFA
+-/
+def convert (M : NFA α σ) {τ} (equiv : σ ≃ τ) : NFA α τ :=
+⟨
+  (λ p a q, M.step (equiv.inv_fun p) a (equiv.inv_fun q)),
+  (λ q, M.start (equiv.inv_fun q)),
+  (λ q, M.accept (equiv.inv_fun q))
+⟩
+
+/- TODO: maybe mark as @simp -/
+theorem convert_correct (M : NFA α σ) {τ} (equiv : σ ≃ τ) : M.accepts = (M.convert equiv).accepts :=
 begin
+  ext,
+  split,
+  { rintros ⟨q, accept, eval⟩,
+    refine ⟨equiv.to_fun q, _, _⟩,
+    { unfold convert,
+      rw set.mem_def at *,
+      simpa,
+    },
+    { clear accept,
+      revert eval,
+      rw ← x.reverse_reverse,
+      induction x.reverse generalizing q,
+      case nil {
+        assume hx,
+        unfold convert,
+        rw set.mem_def at *,
+        simpa,
+      },
+      case cons : a as ih {
+        assume hx,
+        simp at *,
+        rw NFA.mem_step_set at *,
+        rcases hx with ⟨p, mem, step⟩,
+        refine ⟨equiv.to_fun p, ih p mem, _⟩,
+        unfold convert,
+        rw set.mem_def at *,
+        simpa,
+      },
+    },        
+  },
+  { rintros ⟨q, accept, eval⟩,
+    refine ⟨equiv.inv_fun q, accept, _⟩,
+    clear accept,
+    revert eval,
+    rw ← x.reverse_reverse,
+    induction x.reverse generalizing q,
+    case nil {
+      assume hx,
+      exact hx,
+    },
+    case cons : a as ih {
+      assume hx,
+      simp at *,
+      rw NFA.mem_step_set at *,
+      rcases hx with ⟨p, mem, step⟩,
+      exact ⟨equiv.inv_fun p, ih p mem, step⟩,
+    },
+  },
+end
+
+variables
+  (M : NFA α (fin n))
+  [dec_start : decidable_pred M.start]
+  [dec_accept : decidable_pred M.accept]
+  [dec_step : ∀ p a q, decidable (M.step p a q)]
+  (as : list α)
+
+include dec_start dec_accept dec_step
+
+/--
+Convert an NFA with state type `fin n` to the corresponding GNFA.
+
+Note: needs decidability for each of the NFA's functions, and a list of all the elements of the
+alphabet.
+
+TODO: would it be a good idea to make a separate "decidable NFA" structure?
+-/
+def to_GNFA : GNFA α n :=
+⟨
+  λ p q,
+  match (p, q) with
+  | (none, none) := 0
+  | (none, some q) := if M.start q then 1 else 0
+  | (some p, none) := if M.accept p then 1 else 0
+  | (some p, some q) :=
+    list.sum $
+      list.map (λ a, regular_expression.char a) $
+        list.filter (λ a, M.step p a q) as
+  end
+⟩
+
+/- TODO: maybe mark as @simp -/
+theorem to_GNFA_correct (univ : ∀ a, a ∈ as) : M.accepts = (M.to_GNFA as).accepts :=
+begin
+  ext,
+  split,
+  { rintros ⟨q, accept, eval⟩,
+    refine GNFA.accepts.step q _ _ x.append_nil.symm,
+    swap,
+    { rw set.mem_def,
+      unfold to_GNFA,
+      simp,
+      unfold to_GNFA._match_1,
+      rw set.mem_def at accept,
+      simp [accept],
+      exact rfl,
+    },
+    clear accept,
+    revert eval,
+    rw ← x.reverse_reverse,
+    induction x.reverse generalizing q,
+    case nil {
+      assume hx,
+      simp,
+      refine GNFA.trace.start _,
+      unfold to_GNFA,
+      simp,
+      unfold to_GNFA._match_1,
+      rw set.mem_def at hx,
+      simp at hx,
+      simp [hx],
+    },
+    case cons : a as ih {
+      assume hx,
+      simp at *,
+      rw NFA.mem_step_set at hx,
+      rcases hx with ⟨p, mem, step⟩,
+      refine GNFA.trace.step p (ih p mem) _ rfl,
+      rw set.mem_def,
+      unfold to_GNFA,
+      simp,
+      unfold to_GNFA._match_1,
+      rw regular_expression.mem_sum_iff_exists_mem,      
+      refine ⟨regular_expression.char a, _, rfl⟩,
+      simpa [univ],
+    },
+  },
+  { assume hx,
+    cases hx with x step x y z q t step eq,
+    case start { cases step,},
+    unfold to_GNFA at step,
+    rw set.mem_def at step,
+    simp at step,
+    unfold to_GNFA._match_1 at step,
+    by_cases M.accept q,
+    swap, simp [h] at step, cases step,
+    simp [h] at step,
+    cases step,
+    refine ⟨q, h, _⟩,
+    simp at eq, cases eq,
+    clear h eq step,
+    revert t,
+    rw ← x.reverse_reverse,
+    induction x.reverse generalizing q,
+    case nil {
+      assume hx,
+      simp at *,
+      cases hx,
+      case start : x step {
+        unfold to_GNFA at step,
+        rw set.mem_def at step,
+        simp at step,
+        unfold to_GNFA._match_1 at step,
+        by_cases M.start x,
+        exact h,
+        simp [h] at step,
+        cases step,
+      },
+      case step : x y z p t step eq {
+        simp at eq,
+        rw eq.2 at *,
+        unfold to_GNFA at step,
+        rw set.mem_def at step,
+        simp at step,
+        unfold to_GNFA._match_1 at step,
+        rw regular_expression.mem_sum_iff_exists_mem at step,
+        rcases step with ⟨r, mem, matches⟩,
+        simp at mem,
+        rcases mem with ⟨a, _, eq⟩,
+        rw ← eq at matches,
+        cases matches,
+      },
+    },
+    case cons : a as ih {
+      assume hx,
+      simp at *,
+      rw NFA.mem_step_set,
+      cases hx,
+      case start : q step {
+        unfold to_GNFA at step,
+        simp at step,
+        rw set.mem_def at step,
+        unfold to_GNFA._match_1 at step,
+        by_cases M.start q,
+        { simp [h] at step,
+          by_cases as.reverse.append [a] = [],
+          { have h : as.reverse ++ [a] = list.nil := h,
+            rw ← list.reverse_cons a as at h,
+            rw list.reverse_eq_nil at h,
+            contradiction,
+          },
+          { rcases list.exists_cons_of_ne_nil h with ⟨a, as, h⟩,
+            rw h at step,
+            cases step,
+          },
+        },
+        { simp [h] at step,
+          cases step,
+        },
+      },
+      case step : y z p q t step eq {
+        unfold to_GNFA at step,
+        rw set.mem_def at step,
+        simp at step,
+        unfold to_GNFA._match_1 at step,
+        replace eq : as.reverse ++ [a] = y ++ z := eq,
+        rw regular_expression.mem_sum_iff_exists_mem at step,
+        rcases step with ⟨r, mem, matches⟩,
+        simp at mem,
+        rcases mem with ⟨b, ⟨_, step⟩, eq⟩,
+        rw ← eq at matches,
+        cases matches,
+        rw ← list.reverse_inj at eq,
+        simp at eq,
+        rw ← eq.1 at step,
+        refine ⟨p, _, step⟩,
+        rw ← y.reverse_reverse at t,
+        rw ← eq.2 at t,
+        exact ih p t,        
+      },
+    },
+  },
+end
+
+omit dec_start dec_accept dec_step
+
+/--
+Given an NFA with a `fintype` state, there is a regular expression that matches the same language.
+
+TODO:
+ * I'd like to call the NFA parameter `M`, but the name is already taken in the `variables`
+   declaration earlier, so compiler doesn't like it. Is there a way around this besides listing
+   out all the parameters in both of the earlier declarations?
+ * This does not follow the precedent that `to_DFA` and `to_NFA` are both constructive definitions
+   that give back just the resulting machine, and have `to_DFA_correct` and `to_NFA_correct`
+   separately. Change the name? Find some other way?
+-/
+theorem to_regular_expression (M₀ : NFA α σ) [fintype α] [fintype σ] : ∃ (r : regular_expression α), M₀.accepts = r.matches :=
+begin
+  classical,
   rcases fintype.exists_univ_list α with ⟨as, _, univ⟩,
-  let M' := M.convert (fintype.equiv_fin σ),
-  let M'' := @to_GNFA _ _ M' (classical.dec_pred _) (classical.dec_pred _) (λ p a q, classical.dec _) as univ,
-  let r := M''.to_regular_expression,
+  let M₁ := M₀.convert (fintype.equiv_fin σ),
+  let M₂ := M₁.to_GNFA as,
+  let r := M₂.to_regular_expression,
   use r,
   rw ← GNFA.to_regular_expression_correct,
-  rw ← to_GNFA_correct,
+  rw ← to_GNFA_correct _ _ univ,
   rw ← convert_correct,
 end
 
